checkpoint

dafny/top-down/search_clause.dfy
@@ -1,12 +1,30 @@
 include "evar.dfy"
-
+include "definitions.dfy"
 include "std-lib/src/Wrappers.dfy"
 include "std-lib/src/Collections/Sequences/Seq.dfy"
+include "bijective_map.dfy"
 import opened Wrappers
 import opened Seq
+import opened BijectiveMap
 
-datatype SearchClause = SearchClause(name:string, evar_terms:seq<Evar>)
+datatype SearchClause = SearchClause(name:string, evar_terms:seq<Evar>, rule: Rule, bimap:BijectiveMap<VarTerm, Evar>)
 {
+    predicate valid()
+    {
+        rule.head.name == name
+        // Todo something about the body mapping to the rule's body under some evar map
+    }
+    function subst_of() : Substitution
+        ensures rule.head.substitution_concrete(subst_of())
+        ensures (forall clause :: clause in rule.body ==> 
+                        clause.substitution_concrete(subst_of()))
+    {
+        //bimap.l_to_r
+        assume false;
+        map[]
+        // todo something about applying it to an evar_map to get an actual concrete subst out of it
+    }
+
   // predicate is_ground() 
   // {
   //   forall t :: t in terms ==> t.Const?
